Refactoring for the initial env.
Make the repl semantics parameterised over the initial enviroment, and
move everything about the initial env into the "initial" directory.
Ideally, the metatheory, inference, and compiler proofs won't depend at
all on the initial env. This now is true for everything but
compilerProofScript.

compiler/proofs/modLangProofScript.sml
@@ -2333,38 +2333,4 @@ val whole_prog_to_i1_correct = Q.store_thm ("whole_prog_to_i1_correct",
  fs [no_dup_mods_def, no_dup_mods_i1_def, no_dup_top_types_def, no_dup_top_types_i1_def] >>
  metis_tac [prog_to_i1_mods, prog_to_i1_top_types, prog_to_i1_mods_ok, NOT_EVERY]);
 
-val init_mods_def = Define `
-  init_mods = FEMPTY`;
-
-val init_tops_def = Define `
-  init_tops = FEMPTY |++ alloc_defs 0 (MAP FST init_env)`;
-
-val init_genv_def = Define `
-  init_genv =
-    MAP (\(x,v).
-           case v of
-             | Closure _ x e => SOME (Closure_i1 (init_envC,[]) x (exp_to_i1 init_mods (init_tops\\x) e)))
-        init_env`;
-
-val initial_i1_invariant = Q.prove (
-`global_env_inv init_genv init_mods init_tops [] {} init_env ∧
- s_to_i1' init_genv [] []`,
- rw [last (CONJUNCTS v_to_i1_eqns)]
- >- (rw [v_to_i1_eqns, init_tops_def] >>
-     fs [init_env_def, alloc_defs_def] >>
-     rpt (full_case_tac
-          >- (rw [] >>
-              rw [flookup_fupdate_list] >>
-              rw [init_genv_def, Once v_to_i1_cases] >>
-              rw [v_to_i1_eqns] >>
-              rw [init_env_def, DRESTRICT_UNIV] >>
-              metis_tac [])) >>
-     fs [])
- >- rw [v_to_i1_eqns, s_to_i1'_cases]);
-
-val init_to_i1_invariant = Q.store_thm ("init_to_i1_invariant",
-`!count. to_i1_invariant init_genv init_mods init_tops [] init_env (count,[]) (count,[]) {}`,
- rw [to_i1_invariant_def, s_to_i1_cases] >>
- metis_tac [initial_i1_invariant]);
-
 val _ = export_theory ();
