initial/initialProgramScript.sml
@@ -3,36 +3,252 @@ open astTheory bytecodeExtraTheory
 
 val _ = new_theory"initialProgram"
 
-val initial_program_def = Define `
-initial_program =
-   Dlet (Pcon NONE [Pvar "ref";
-                    Pvar "!";
-                    Pvar "~";
-                    Pvar ":=";
-                    Pvar "=";
-                    Pvar ">=";
-                    Pvar "<=";
-                    Pvar ">";
-                    Pvar "<";
-                    Pvar "mod";
-                    Pvar "div";
-                    Pvar "*";
-                    Pvar "-";
-                    Pvar "+"])
-        (Con NONE [(Fun "x" (Uapp Opref (Var(Short"x"))));
-                   (Fun "x" (Uapp Opderef (Var(Short"x"))));
-                   (Fun "x" (App (Opn Minus) (Lit (IntLit 0)) (Var(Short"x"))));
-                   (Fun "x" (Fun"y"(App Opassign (Var(Short"x"))(Var(Short"y")))));
-                   (Fun "x" (Fun"y"(App Equality(Var(Short"x"))(Var(Short"y")))));
-                   (Fun "x" (Fun"y"(App(Opb Geq)(Var(Short"x"))(Var(Short"y")))));
-                   (Fun "x" (Fun"y"(App(Opb Leq)(Var(Short"x"))(Var(Short"y")))));
-                   (Fun "x" (Fun"y"(App(Opb Gt)(Var(Short"x"))(Var(Short"y")))));
-                   (Fun "x" (Fun"y"(App(Opb Lt)(Var(Short"x"))(Var(Short"y")))));
-                   (Fun "x" (Fun"y"(App(Opn Modulo)(Var(Short"x"))(Var(Short"y")))));
-                   (Fun "x" (Fun"y"(App(Opn Divide)(Var(Short"x"))(Var(Short"y")))));
-                   (Fun "x" (Fun"y"(App(Opn Times)(Var(Short"x"))(Var(Short"y")))));
-                   (Fun "x" (Fun"y"(App(Opn Minus)(Var(Short"x"))(Var(Short"y")))));
-                   (Fun "x" (Fun"y"(App(Opn Plus)(Var(Short"x"))(Var(Short"y")))))])`;
+(* From type inference *)
+
+val infer_init_thm = Q.store_thm ("infer_init_thm",
+`infer_sound_invariant [] ([],[]) init_type_env ∧
+ (convert_decls init_infer_decls = init_decls) ∧
+ (convert_menv [] = []) ∧
+ (bind_var_list2 (convert_env2 init_type_env) Empty = init_tenv)`,
+rw [check_t_def, check_menv_def, check_cenv_def, check_env_def, init_type_env_def,
+    Infer_Tfn_def, Infer_Tint_def, Infer_Tbool_def, Infer_Tunit_def, 
+    Infer_Tref_def, init_tenv_def, bind_var_list2_def, convert_env2_def,
+    convert_t_def, convert_menv_def, bind_tenv_def, check_flat_cenv_def,
+    infer_sound_invariant_def, init_decls_def, init_infer_decls_def, 
+    convert_decls_def]);
+
+(* ----------------- *)
+
+(* from type soundness *)
+
+val to_ctMap_list_def = Define `
+to_ctMap_list tenvC =  
+  flat_to_ctMap_list (SND tenvC) ++ FLAT (MAP (\(mn, tenvC). flat_to_ctMap_list tenvC) (FST tenvC))`;
+
+val to_ctMap_def = Define `
+  to_ctMap tenvC = FEMPTY |++ REVERSE (to_ctMap_list tenvC)`;
+ 
+val thms = [to_ctMap_def, to_ctMap_list_def, init_tenvC_def, emp_def, flat_to_ctMap_def, flat_to_ctMap_list_def]; 
+
+val to_ctMap_init_tenvC = 
+  SIMP_CONV (srw_ss()) thms ``to_ctMap init_tenvC``;
+
+val type_check_v_tac = 
+ rw [Once type_v_cases, type_env_eqn2] >>
+ MAP_EVERY qexists_tac [`[]`, `init_tenvC`, `Empty`] >>
+ rw [tenvM_ok_def, type_env_eqn2, check_freevars_def, Once consistent_mod_cases] >>
+ NTAC 10 (rw [Once type_e_cases, num_tvs_def, bind_tvar_def,
+              t_lookup_var_id_def, check_freevars_def, lookup_tenv_def, bind_tenv_def,
+              deBruijn_inc_def, deBruijn_subst_def,
+              METIS_PROVE [] ``(?x. P ∧ Q x) = (P ∧ ?x. Q x)``,
+              LENGTH_NIL_SYM, type_op_cases, type_uop_cases]);
+
+val initial_type_sound_invariants = Q.store_thm ("initial_type_sound_invariant",
+`type_sound_invariants (init_decls,[],init_tenvC,init_tenv,init_type_decs,[],init_envC,init_env,[])`,
+ rw [type_sound_invariants_def] >>
+ MAP_EVERY qexists_tac [`to_ctMap init_tenvC`, `[]`, `init_decls`, `[]`, `init_tenvC`] >>
+ `consistent_con_env (to_ctMap init_tenvC) init_envC init_tenvC`
+         by (rw [to_ctMap_init_tenvC] >>
+             rw [consistent_con_env_def, init_envC_def, init_tenvC_def, emp_def, tenvC_ok_def, 
+                 flat_tenvC_ok_def, check_freevars_def, ctMap_ok_def, FEVERY_ALL_FLOOKUP,
+                 flookup_fupdate_list, lookup_con_id_def]
+             >- (every_case_tac >>
+                 fs [] >>
+                 rw [check_freevars_def])
+             >- (Cases_on `cn` >>
+                 fs [id_to_n_def] >>
+                 every_case_tac >>
+                 fs [])
+             >- (Cases_on `cn` >>
+                 fs [id_to_n_def] >>
+                 every_case_tac >>
+                 fs [])) >>
+ rw []
+ >- (rw [consistent_decls_def, init_type_decs_def, init_decls_def, RES_FORALL] >>
+     every_case_tac >>
+     fs [])
+ >- (rw [consistent_ctMap_def, to_ctMap_init_tenvC, init_decls_def, RES_FORALL] >>
+     PairCases_on `x` >>
+     fs [] >>
+     every_case_tac >>
+     fs [FDOM_FUPDATE_LIST])
+ >- rw [ctMap_has_exns_def, to_ctMap_init_tenvC, flookup_fupdate_list]
+ >- rw [tenvM_ok_def]
+ >- rw [tenvM_ok_def]
+ >- rw [Once type_v_cases]
+ >- (rw [init_env_def, emp_def, init_tenv_def, type_env_eqn2] >>
+     type_check_v_tac)
+ >- rw [type_s_def, store_lookup_def] 
+ >- rw [weakM_def]
+ >- rw [weakC_refl]
+ >- rw [decls_ok_def, init_decls_def, decls_to_mods_def, SUBSET_DEF, GSPECIFICATION]
+ >- metis_tac [weak_decls_refl]
+ >- rw [init_decls_def, weak_decls_only_mods_def]);
+
+(* ------------------- *)
+
+(* from conLang *)
+
+val init_tagenv_state : (nat * tag_env * map nat (conN * tid_or_exn))
+let init_tagenv_state =
+  (8,
+   (Map.empty,
+    Map.fromList [("Div", (div_tag, Just (TypeExn (Short "Div")))); 
+                  ("Bind", (bind_tag,Just (TypeExn (Short "Bind")))); 
+                  ("Eq", (eq_tag, Just (TypeExn (Short "Eq")))); 
+                  ("::", (cons_tag, Just (TypeId (Short "list"))));
+                  ("nil", (nil_tag, Just (TypeId (Short "list"))));
+                  ("SOME", (some_tag, Just (TypeId (Short "option"))));
+                  ("NONE", (none_tag, Just (TypeId (Short "option"))))]),
+   Map.fromList [(div_tag, ("Div", TypeExn (Short "Div"))); 
+                 (bind_tag, ("Bind", TypeExn (Short "Bind"))); 
+                 (eq_tag, ("Eq", TypeExn (Short "Eq"))); 
+                 (cons_tag, ("::", TypeId (Short "list")));
+                 (nil_tag, ("nil", TypeId (Short "list")));
+                 (some_tag, ("SOME", TypeId (Short "option")));
+                 (none_tag, ("NONE", TypeId (Short "option")))])
+
+val init_exh : exh_ctors_env
+let init_exh =
+  Map.fromList
+    [(Short "list", nat_set_from_list [cons_tag; nil_tag]);
+     (Short "option", nat_set_from_list [some_tag; none_tag])]
+
+(* ----------------- *)
+
+(* from compiler.lem *)
+
+let init_compiler_state =
+  <| next_global = 0
+   ; globals_env = (Map.empty, Map.empty)
+   ; contags_env = init_tagenv_state
+   ; exh = init_exh
+   ; rnext_label = 0
+   |>
+
+(* ----------------- *)
+
+(* from modLangProof *)
+
+val init_mods_def = Define `
+  init_mods = FEMPTY`;
+
+val init_tops_def = Define `
+  init_tops = FEMPTY |++ alloc_defs 0 (MAP FST init_env)`;
+
+val init_genv_def = Define `
+  init_genv =
+    MAP (\(x,v).
+           case v of
+             | Closure _ x e => SOME (Closure_i1 (init_envC,[]) x (exp_to_i1 init_mods (init_tops\\x) e)))
+        init_env`;
+
+val initial_i1_invariant = Q.prove (
+`global_env_inv init_genv init_mods init_tops [] {} init_env ∧
+ s_to_i1' init_genv [] []`,
+ rw [last (CONJUNCTS v_to_i1_eqns)]
+ >- (rw [v_to_i1_eqns, init_tops_def] >>
+     fs [init_env_def, alloc_defs_def] >>
+     rpt (full_case_tac
+          >- (rw [] >>
+              rw [flookup_fupdate_list] >>
+              rw [init_genv_def, Once v_to_i1_cases] >>
+              rw [v_to_i1_eqns] >>
+              rw [init_env_def, DRESTRICT_UNIV] >>
+              metis_tac [])) >>
+     fs [])
+ >- rw [v_to_i1_eqns, s_to_i1'_cases]);
+
+val init_to_i1_invariant = Q.store_thm ("init_to_i1_invariant",
+`!count. to_i1_invariant init_genv init_mods init_tops [] init_env (count,[]) (count,[]) {}`,
+ rw [to_i1_invariant_def, s_to_i1_cases] >>
+ metis_tac [initial_i1_invariant]);
+
+(* ----------------- *)
+
+(* from conLangProof *)
+val init_gtagenv_def = Define `
+init_gtagenv =
+  FEMPTY |++ [(("NONE",TypeId (Short "option")), (none_tag, 0));
+              (("SOME",TypeId (Short "option")), (some_tag, 1));
+              (("nil",TypeId (Short "list")), (nil_tag, 0:num));
+              (("::",TypeId (Short "list")), (cons_tag, 2));
+              (("Bind",TypeExn (Short "Bind")), (bind_tag,0));
+              (("Div",TypeExn (Short "Div")), (div_tag,0));
+              (("Eq",TypeExn (Short "Eq")), (eq_tag,0))]`;
+
+val initial_i2_invariant = Q.store_thm ("initial_i2_invariant",
+`!ck.
+  to_i2_invariant
+    {}
+    (IMAGE SND (FDOM init_gtagenv))
+    init_envC
+    init_exh
+    init_tagenv_state
+    init_gtagenv
+    (ck,[]) (ck,[])
+    [] []`,
+ rw [to_i2_invariant_def, s_to_i2_cases, v_to_i2_eqns, s_to_i2'_cases]
+ >- EVAL_TAC
+ >- (simp[EXISTS_PROD] >>
+     pop_assum mp_tac >> EVAL_TAC >> simp[] >>
+     metis_tac[] )
+ >- EVAL_TAC
+ >- (rw [cenv_inv_def, envC_tagged_def, exhaustive_env_correct_def]
+     >- (fs [initialEnvTheory.init_envC_def] >>
+         cases_on `cn` >>
+         fs [id_to_n_def] >>
+         fs [lookup_con_id_def, emp_def, nil_tag_def, emp_def, cons_tag_def,
+             bind_tag_def, div_tag_def, eq_tag_def] >>
+         EVAL_TAC >> rw[] >> fs[])
+     >- (
+       fs[init_exh_def,IN_FRANGE_FLOOKUP,flookup_fupdate_list] >>
+       every_case_tac >> fs[] >> rw[] >>
+       rw[nat_set_from_list_def] >>
+       rpt (match_mp_tac sptreeTheory.wf_insert) >>
+       rw[sptreeTheory.wf_def] )
+     >- (fs [FDOM_FUPDATE_LIST, init_exh_def, init_gtagenv_def] >>
+         rw [flookup_fupdate_list] >>
+         every_case_tac >>
+         rw[nat_set_from_list_def,domain_nat_set_from_list])
+     >- (rw [gtagenv_wf_def, has_exns_def, init_gtagenv_def, flookup_fupdate_list] >>
+         rw[nil_tag_def,cons_tag_def,eq_tag_def,tuple_tag_def,bind_tag_def,div_tag_def,none_tag_def,some_tag_def] >>
+         pop_assum mp_tac >>
+         rw[nil_tag_def,cons_tag_def,eq_tag_def,tuple_tag_def,bind_tag_def,div_tag_def,none_tag_def,some_tag_def] >>
+         pop_assum mp_tac >>
+         rw[nil_tag_def,cons_tag_def,eq_tag_def,tuple_tag_def,bind_tag_def,div_tag_def,none_tag_def,some_tag_def]))
+ >- (rw [alloc_tags_invariant_def, init_gtagenv_def, FDOM_FUPDATE_LIST, get_next_def,
+         tuple_tag_def, init_tagenv_state_def, flookup_fupdate_list, get_tagacc_def] >>
+     pop_assum mp_tac >>
+     srw_tac [ARITH_ss] [nil_tag_def,cons_tag_def,eq_tag_def,tuple_tag_def, bind_tag_def, div_tag_def,none_tag_def,some_tag_def]));
+(* ----------------- *)
+
+(* from compilerProof *)
+val env_rs_empty = store_thm("env_rs_empty",
+  ``∀envs s cs genv rd grd bs ck.
+    bs.stack = [] ∧ bs.globals = [] ∧ FILTER is_Label bs.code = [] ∧
+    (∀n. bs.clock = SOME n ⇒ n = ck) ∧ envs = ([],init_envC,[]) ∧
+    s = ((ck,[]),IMAGE SND (FDOM init_gtagenv),{}) ∧
+    grd = ([],init_gtagenv,rd) ∧
+    rd.sm = [] ∧ rd.cls = FEMPTY ∧ cs = init_compiler_state ⇒
+    env_rs envs s grd cs bs``,
+  rpt gen_tac >>
+  simp[env_rs_def,to_i1_invariant_def,to_i2_invariant_def] >>
+  strip_tac >>
+  conj_tac >- (EVAL_TAC >> simp[]) >>
+  conj_tac >- (EVAL_TAC >> simp[]) >>
+  rw[init_compiler_state_def,get_tagenv_def,cenv_inv_def] >>
+  rw[Once v_to_i1_cases] >> rw[Once v_to_i1_cases] >>
+  rw[Once s_to_i1_cases] >> rw[Once s_to_i1'_cases] >> rw[Once v_to_i1_cases] >>
+  simp[Once s_to_i2_cases] >> simp[Once s_to_i2'_cases] >> simp[Once v_to_i2_cases] >>
+  simp[Cenv_bs_def,env_renv_def,s_refs_def,good_rd_def,FEVERY_ALL_FLOOKUP] >>
+  simp[all_vlabs_csg_def,vlabs_csg_def,closed_vlabs_def] >>
+  conj_tac >- EVAL_TAC >>
+  Q.ISPEC_THEN`ck`assume_tac initial_i2_invariant >>
+  fs[to_i2_invariant_def] >>
+  fs[cenv_inv_def])
+
+(* ----------------- *)
 
 val empty_bc_state_def = Define `
   empty_bc_state = <| stack := []; code := []; pc := 0; refs := FEMPTY;
